\chapter*{Ejercicio 3}
% \section*{Ejercicio 3}

A partir de la siguiente gram√°tica para expresiones proposicionales:

\[
E \to T \mid \neg E \mid E \land E \mid E \lor E \mid E \to E \mid (E)
\]
\[
T \to p \mid q \mid r \mid a \mid b \mid c \mid d
\]

\subsection*{a) $p \to q$}

\vspace*{\fill}
\begin{center}
\[
\begin{array}{c}
     \rightarrow \\
    / \ \backslash \\
   p   \quad  q 
\end{array}
\]
\end{center}
\vspace*{\fill}

\subsection*{b) $\neg(p \lor q)$}

\vspace*{\fill}
\begin{center}
\[
\begin{array}{c}
      \neg \\
      | \\
      \lor \\
     / \ \backslash \\
    p   \quad  q 
\end{array}
\]
\end{center}
\vspace*{\fill}

\subsection*{c) $(a \land b) \lor c \to (a \land d)$}

\vspace*{\fill}
\begin{center}
\[
\begin{array}{c}
      \rightarrow \\
      / \quad\ \quad \backslash \\
      \lor   \quad \quad \quad \land  \\
    / \ \backslash \quad\quad \quad / \ \backslash \\
   \land   \quad c \quad \quad   a \quad b\\
  / \ \backslash \quad \quad \quad \quad  \quad\\
 a   \quad  b  \quad \quad \quad\quad \quad
\end{array}
\]
\end{center}
\vspace*{\fill}

\subsection*{d) $(p \to a) \to (a \lor \neg b)$}

\vspace*{\fill}
\begin{center}
\[
\begin{array}{c}
       \rightarrow \\
      / \quad \ \backslash \\
     \rightarrow   \quad  \lor \\
    / \ \backslash \quad / \ \backslash\\
   p   \quad  a   \quad a \quad \neg\\
               \quad   | \\
                \quad   b
\end{array}
\]
\end{center}
\vspace*{\fill}

\subsection*{e) $\neg p \land \neg q \lor r$}

\vspace*{\fill}
\begin{center}
\[
\begin{array}{c}
      \lor \\
     / \ \backslash \\
    \land   \quad  r \\
   /  \ \backslash \quad \\
  \neg  \quad  \neg \quad \\
  | \quad \quad| \quad\\
  p \quad  \quad q \quad
\end{array}
\]
\end{center}
\vspace*{\fill}

\subsection*{f) $\neg a \to (b \land \neg c) \leftrightarrow \neg d$}

\vspace*{\fill}
\begin{center}
\[
\begin{array}{c}
      \leftrightarrow \\
     / \quad \ \backslash \\
    \to   \quad\quad  \neg \quad \\
   / \quad\ \backslash \quad \quad | \quad\\
   \neg    \quad \quad \land \quad d \quad \quad\\
      |\quad \quad       / \ \backslash \quad \quad \quad\\
      a\quad  \quad    b   \quad \neg  \quad \quad \\
      | \quad\\
      c \quad
\end{array}
\]
\end{center}
\vspace*{\fill}

\vspace*{\fill}